Launchbury/ResourcedDenotational.thy
@@ -4,28 +4,22 @@ begin
 
 type_synonym CEnv = "var f\<rightharpoonup> CValue"
 
-interpretation cont_semantic_domain
-  "\<lambda> f . \<Lambda> r. CFn\<cdot>(\<Lambda> v. C_restr \<cdot> r \<cdot> (f\<cdot> (C_restr \<cdot> r \<cdot> v)))"
-  "\<lambda>x y. (\<Lambda> r. (x\<cdot>r \<down>CFn C_restr\<cdot>r\<cdot>y)\<cdot>r)"
-  "\<lambda> x. C_case \<cdot> x"
-  by unfold_locales simp_all
-declare cont_semantic_domain_conts[simp del]
+interpretation semantic_domain
+  "\<Lambda> f . \<Lambda> r. CFn\<cdot>(\<Lambda> v. C_restr \<cdot> r \<cdot> (f\<cdot> (C_restr \<cdot> r \<cdot> v)))"
+  "\<Lambda> x y. (\<Lambda> r. (x\<cdot>r \<down>CFn C_restr\<cdot>r\<cdot>y)\<cdot>r)"
+  "\<Lambda> x. (\<Lambda> (C\<cdot>r). x \<cdot> r)".
 
-abbreviation CESem ("\<N>\<lbrakk> _ \<rbrakk>\<^bsub>_\<^esub>"  [60,60] 60) where "\<N>\<lbrakk> e \<rbrakk>\<^bsub>\<rho>\<^esub> \<equiv> AESem e \<rho>"
+abbreviation CESem_syn ("\<N>\<lbrakk> _ \<rbrakk>\<^bsub>_\<^esub>"  [60,60] 60) where "\<N>\<lbrakk> e \<rbrakk>\<^bsub>\<rho>\<^esub> \<equiv> AESem e \<cdot> \<rho>"
+abbreviation CHSem_syn ("\<N>\<lbrace>_\<rbrace>_"  [60,60] 60) where "\<N>\<lbrace>\<Gamma>\<rbrace>\<rho> \<equiv> UHSem \<Gamma> \<cdot> \<rho>"
+abbreviation CHSem_fempty  ("\<N>\<lbrace>_\<rbrace>"  [60] 60) where "\<N>\<lbrace>\<Gamma>\<rbrace> \<equiv> \<N>\<lbrace>\<Gamma>\<rbrace>fempty"
 
 (* The same, but with some beta_cfun's and eta_cfuns resolved.*)
 lemma CESem_simps:
   "\<N>\<lbrakk> Lam [x]. e \<rbrakk>\<^bsub>\<rho>\<^esub> = (\<Lambda> (C\<cdot>r). (CFn\<cdot>(\<Lambda> v. C_restr\<cdot>r\<cdot>(\<N>\<lbrakk>e\<rbrakk>\<^bsub>\<rho>(x f\<mapsto> C_restr\<cdot>r\<cdot>v)\<^esub>))))"
-  "\<N>\<lbrakk> App e x \<rbrakk>\<^bsub>\<rho>\<^esub>    =  (\<Lambda> (C\<cdot>r). ((\<N>\<lbrakk>e\<rbrakk>\<^bsub>\<rho>\<^esub>)\<cdot>r \<down>CFn C_restr\<cdot>r\<cdot>(\<rho> f!\<^sub>\<bottom> x))\<cdot>r)"
-  "\<N>\<lbrakk> Var x \<rbrakk>\<^bsub>\<rho>\<^esub>      = (\<Lambda> (C \<cdot> r). (\<rho> f!\<^sub>\<bottom> x) \<cdot> r)"
-  "set (bn as) \<sharp>* \<rho> \<Longrightarrow>
-  \<N>\<lbrakk> Let as body \<rbrakk>\<^bsub>\<rho>\<^esub> = (\<Lambda> (C \<cdot> r). (\<N>\<lbrakk>body\<rbrakk>\<^bsub>has_ESem.UHSem CESem (asToHeap as) \<rho>\<^esub>) \<cdot> r)"
-  by (simp_all add: eta_cfun)
-
-
-abbreviation CHSem_syn ("\<N>\<lbrace>_\<rbrace>_"  [60,60] 60) where "\<N>\<lbrace>\<Gamma>\<rbrace>\<rho> \<equiv> UHSem \<Gamma> \<rho>"
-abbreviation CHSem_fempty  ("\<N>\<lbrace>_\<rbrace>"  [60] 60) where "\<N>\<lbrace>\<Gamma>\<rbrace> \<equiv> \<N>\<lbrace>\<Gamma>\<rbrace>fempty"
-
+  "\<N>\<lbrakk> App e x \<rbrakk>\<^bsub>\<rho>\<^esub>    = (\<Lambda> (C\<cdot>r). ((\<N>\<lbrakk>e\<rbrakk>\<^bsub>\<rho>\<^esub>)\<cdot>r \<down>CFn C_restr\<cdot>r\<cdot>(\<rho> f!\<^sub>\<bottom> x))\<cdot>r)"
+  "\<N>\<lbrakk> Var x \<rbrakk>\<^bsub>\<rho>\<^esub>      = (\<Lambda> (C\<cdot>r). (\<rho> f!\<^sub>\<bottom> x) \<cdot> r)"
+  "\<N>\<lbrakk> Let as body \<rbrakk>\<^bsub>\<rho>\<^esub> = (\<Lambda> (C \<cdot> r). (\<N>\<lbrakk>body\<rbrakk>\<^bsub>\<N>\<lbrace>asToHeap as\<rbrace>\<rho>\<^esub>) \<cdot> r)"
+  by (simp_all)
 
 lemma CESem_bot[simp]:"(\<N>\<lbrakk> e \<rbrakk>\<^bsub>\<sigma>\<^esub>)\<cdot>\<bottom> = \<bottom>"
   by (nominal_induct e avoiding: \<sigma> rule: exp_assn.strong_induct(1)) auto
