Launchbury/CorrectnessResourced.thy
@@ -32,7 +32,7 @@ case (Application y \<Gamma> e x L \<Delta> \<Theta> z e' \<rho>)
     using fun_belowD[OF Application.hyps(11)[OF hyp1]]
     by (fastforce intro: monofun_cfun_arg monofun_cfun_fun monofun_LAM)
   also have "\<dots> = (\<Lambda> (C\<cdot>r). (((\<Lambda> (C \<cdot> r). CFn \<cdot> (\<Lambda> v. C_restr\<cdot>r\<cdot>(\<N>\<lbrakk> e' \<rbrakk>\<^bsub>(\<N>\<lbrace>\<Delta>\<rbrace>\<rho>)(y f\<mapsto> C_restr\<cdot>r\<cdot>v)\<^esub>)))) \<cdot> r \<down>CFn C_restr\<cdot>r\<cdot>(\<N>\<lbrace>\<Delta>\<rbrace>\<rho> f!\<^sub>\<bottom> x)) \<cdot> r)"
-    by (simp add: Rep_cfun_inverse)
+    by simp
   also have "\<dots> \<sqsubseteq> (\<Lambda> (C\<cdot>r). ((CFn \<cdot> (\<Lambda> v. C_restr\<cdot>r\<cdot>(\<N>\<lbrakk> e' \<rbrakk>\<^bsub>(\<N>\<lbrace>\<Delta>\<rbrace>\<rho>)(y f\<mapsto> C_restr\<cdot>r\<cdot>v)\<^esub>))) \<down>CFn C_restr\<cdot>r\<cdot>(\<N>\<lbrace>\<Delta>\<rbrace>\<rho> f!\<^sub>\<bottom> x)) \<cdot> r)"
     apply (rule cfun_belowI)
     apply (case_tac xa, simp)
