Launchbury/HasESem.thy
@@ -3,9 +3,9 @@ imports "Nominal-HOLCF" "FMap-HOLCF" "HOLCF-Join"
 begin
 
 locale has_ESem =
-  fixes ESem :: "'exp::pt \<Rightarrow> 'var::{cont_pt,at_base} f\<rightharpoonup> 'value \<Rightarrow> 'value::{pure_cpo,Nonempty_Meet_cpo,pcpo}"  ("\<lbrakk> _ \<rbrakk>\<^bsub>_\<^esub>"  [60,60] 60)
-
-locale has_cont_ESem = has_ESem +
-  assumes ESem_cont: "\<And> e. cont (ESem e)"
+  fixes ESem :: "'exp::pt \<Rightarrow> 'var::{cont_pt,at_base} f\<rightharpoonup> 'value \<rightarrow> 'value::{pure_cpo,Nonempty_Meet_cpo,pcpo}" 
+begin
+  abbreviation AESem_syn ("\<lbrakk> _ \<rbrakk>\<^bsub>_\<^esub>"  [60,60] 60) where "\<lbrakk>e\<rbrakk>\<^bsub>\<rho>\<^esub> \<equiv> ESem e \<cdot> \<rho>"
+end
 
 end
